@prefix tm:	<https://w3id.org/transportmode#> .
@prefix foaf: 	<http://xmlns.com/foaf/0.1/>.
@prefix wgs84:	<http://www.w3.org/2003/01/geo/wgs84_pos#>.
@prefix cc: 	<http://creativecommons.org/ns#>.
@prefix rdfs:	<http://www.w3.org/2000/01/rdf-schema#>.
@prefix dct: 	<http://purl.org/dc/terms/>.
@prefix vann: 	<http://purl.org/vocab/vann/>.
@prefix rdf: 	<http://www.w3.org/1999/02/22-rdf-syntax-ns#>.
@prefix skos: 	<http://www.w3.org/2004/02/skos/core#>.

<https://w3id.org/transportmode> a foaf:Document;
	foaf:primaryTopic tm:TransportMode.

tm:transportMode a rdfs:Property;
	skos:definition "Links to the kind of transport mode being used.";
	rdfs:label "Transport Mode"@en;
	rdfs:range tm:TransportMode.

tm:TransportMode a skos:ConceptScheme; 
	skos:prefLabel "Transport Mode"@en ;
	skos:definition "The transport mode expresses the way which a person was moving from one place to another.";
	cc:license <https://creativecommons.org/licenses/by/4.0/> ;
	rdfs:comment "The transport mode expresses the way which a person was moving from one place to another.";
	rdfs:label "Transport Mode"@en;
	vann:preferredNamespacePrefix "tm" ;
	vann:preferredNamespaceUri <https://w3id.org/transportmode#> ;
	dct:creator <https://data.knows.idlab.ugent.be/person/woslabbi/#me> ;
	dct:creator <https://data.knows.idlab.ugent.be/person/SindhuVasireddy/#me> ;
	dct:creator <https://pietercolpaert.be/#me> ;
	dct:issued "2022-06-10"^^xsd:date ;
	dct:modified "2022-06-14"^^xsd:date .

tm:Walking a skos:Concept; 
	skos:inScheme tm:TransportMode;
	skos:definition "This transport mode expresses that a person is walking.";
	skos:prefLabel "Walking"@en.

tm:Bicycling a skos:Concept; 
	skos:inScheme tm:TransportMode;
	skos:definition "This transport mode expresses that a person is bicycling.";
	skos:prefLabel "Bicycling"@en.
	
tm:CarDriving a skos:Concept; 
	skos:inScheme tm:TransportMode;
	skos:definition "This transport mode expresses that a person is driving a car.";
	skos:prefLabel "Car Driving"@en.
	